CleanQ/CleanQ_SetModel.thy
@@ -610,22 +610,33 @@ lemma
 
 
 (* ==================================================================================== *)
-subsection \<open>STUFF\<close>
+subsection \<open>Pre- and post- conditions\<close>
 (* ==================================================================================== *)
 
 definition CleanQ_Set_deq_x_pre :: "'a set \<Rightarrow> 'a \<Rightarrow> ('a CleanQ_Set_State, 'a CleanQ_Set_State) Semantic.xstate set"
-  where "CleanQ_Set_deq_x_pre K b = Semantic.Normal ` { rb. I1 rb K \<and> I2 rb \<and> b \<in> TXY rb }"
+  where "CleanQ_Set_deq_x_pre K b = Semantic.Normal ` { rb. I1 rb K \<and> I2 rb \<and> b \<in> TYX rb }"
 
 definition CleanQ_Set_deq_x_post :: "'a set \<Rightarrow> 'a \<Rightarrow> ('a CleanQ_Set_State, 'a CleanQ_Set_State) Semantic.xstate set"
   where "CleanQ_Set_deq_x_post K b = Semantic.Normal ` { rb. I1 rb K \<and> I2 rb \<and> b \<in> SX rb }"
 
+definition CleanQ_Set_deq_y_pre :: "'a set \<Rightarrow> 'a \<Rightarrow> ('a CleanQ_Set_State, 'a CleanQ_Set_State) Semantic.xstate set"
+  where "CleanQ_Set_deq_y_pre K b = Semantic.Normal ` { rb. I1 rb K \<and> I2 rb \<and> b \<in> TXY rb }"
 
-definition CleanQ_Set_State_enqueuex_pre :: "'a set \<Rightarrow> 'a \<Rightarrow> ('a CleanQ_Set_State, 'a CleanQ_Set_State) Semantic.xstate set"
-  where "CleanQ_Set_State_enqueuex_pre K b = Semantic.Normal ` { rb. I1 rb K \<and> I2 rb \<and> b \<in> SX rb }"
+definition CleanQ_Set_deq_y_post :: "'a set \<Rightarrow> 'a \<Rightarrow> ('a CleanQ_Set_State, 'a CleanQ_Set_State) Semantic.xstate set"
+  where "CleanQ_Set_deq_y_post K b = Semantic.Normal ` { rb. I1 rb K \<and> I2 rb \<and> b \<in> SY rb }"
 
-definition CleanQ_Set_State_enqueuex_post :: "'a set \<Rightarrow> 'a \<Rightarrow> ('a CleanQ_Set_State, 'a CleanQ_Set_State) Semantic.xstate set"
-  where "CleanQ_Set_State_enqueuex_post K b = Semantic.Normal ` { rb. I1 rb K \<and> I2 rb \<and> b \<in> TXY rb }"
 
+definition CleanQ_Set_enq_x_pre :: "'a set \<Rightarrow> 'a \<Rightarrow> ('a CleanQ_Set_State, 'a CleanQ_Set_State) Semantic.xstate set"
+  where "CleanQ_Set_enq_x_pre K b = Semantic.Normal ` { rb. I1 rb K \<and> I2 rb \<and> b \<in> SX rb }"
+
+definition CleanQ_Set_enq_x_post :: "'a set \<Rightarrow> 'a \<Rightarrow> ('a CleanQ_Set_State, 'a CleanQ_Set_State) Semantic.xstate set"
+  where "CleanQ_Set_enq_x_post K b = Semantic.Normal ` { rb. I1 rb K \<and> I2 rb \<and> b \<in> TXY rb }"
+
+definition CleanQ_Set_enq_y_pre :: "'a set \<Rightarrow> 'a \<Rightarrow> ('a CleanQ_Set_State, 'a CleanQ_Set_State) Semantic.xstate set"
+  where "CleanQ_Set_enq_y_pre K b = Semantic.Normal ` { rb. I1 rb K \<and> I2 rb \<and> b \<in> SY rb }"
+
+definition CleanQ_Set_enq_y_post :: "'a set \<Rightarrow> 'a \<Rightarrow> ('a CleanQ_Set_State, 'a CleanQ_Set_State) Semantic.xstate set"
+  where "CleanQ_Set_enq_y_post K b = Semantic.Normal ` { rb. I1 rb K \<and> I2 rb \<and> b \<in> TYX rb }"
 
 (*<*)
 end
