CleanQ/CleanQ_SetListRefinement.thy
@@ -1,0 +1,65 @@
+(*
+ * Copyright (c) 2020, CleanQ Project - Systems Group, ETH Zurich
+ * All rights reserved.
+ *
+ * This software may be distributed and modified according to the terms of
+ * the BSD 2-Clause license. Note that NO WARRANTY is provided.
+ *
+ * See "LICENSE" for details.
+ *
+ * SPDX-License-Identifier: BSD-2-Clause
+ *)
+
+
+
+theory CleanQ_SetListRefinement imports 
+  "../Refinements"
+  CleanQ_SetModel
+  CleanQ_ListModel
+begin
+
+
+definition sr_set_list :: "'a CleanQ_List_State \<Rightarrow> 'a CleanQ_Set_State"
+  where "sr_set_list st_c = \<lparr>SX = lSX st_c, SY = lSY st_c, 
+                             TXY = set (lTXY st_c), TYX = set (lTYX st_c)\<rparr>"
+
+definition fr_id :: "'a CleanQ_List_State \<Rightarrow> 'a CleanQ_Set_State"
+  where "fr_id = sr_set_list"
+
+lemma
+  CleanQ_setListRefinement_enq_x: "((\<Gamma>a, CleanQ_Set_enq_x_pre K buf, Language.Basic (CleanQ_Set_enq_x buf)), 
+                               (\<Gamma>c, CleanQ_List_enq_x_pre K buf, Language.Basic (CleanQ_List_enq_x buf)))
+                               \<in> refinement_s (separable_lift sr_set_list fr_id)"
+apply(rule refinement_s_BasicI) (* Problem applying this after unfolding*)
+  unfolding separable_lift_def sr_set_list_def CleanQ_Set_enq_x_def CleanQ_Set_enq_x_pre_def CleanQ_List_enq_x_def
+  CleanQ_List_enq_x_pre_def
+  by(auto)
+
+lemma
+  CleanQ_setListRefinement_enq_y: "((\<Gamma>a, CleanQ_Set_enq_y_pre K buf, Language.Basic (CleanQ_Set_enq_y buf)), 
+                               (\<Gamma>c, CleanQ_List_enq_y_pre K buf, Language.Basic (CleanQ_List_enq_y buf)))
+                               \<in> refinement_s (separable_lift sr_set_list fr_id)"
+apply(rule refinement_s_BasicI) (* Problem applying this after unfolding*)
+  unfolding separable_lift_def sr_set_list_def  CleanQ_Set_enq_y_def CleanQ_Set_enq_y_pre_def CleanQ_List_enq_y_def
+  CleanQ_List_enq_y_pre_def
+  by(auto)
+
+lemma
+  CleanQ_setListRefinement_deq_x: "((\<Gamma>a, CleanQ_Set_deq_x_pre K buf, Language.Basic (CleanQ_Set_deq_x buf)), 
+                               (\<Gamma>c, CleanQ_List_deq_x_pre K buf, Language.Basic (CleanQ_List_deq_x buf)))
+                               \<in> refinement_s (separable_lift sr_set_list fr_id)"
+apply(rule refinement_s_BasicI) (* Problem applying this after unfolding*)
+  unfolding separable_lift_def sr_set_list_def CleanQ_Set_deq_x_def CleanQ_Set_deq_x_pre_def CleanQ_List_deq_x_def
+  CleanQ_List_deq_x_pre_def
+  by(auto)
+
+lemma
+  CleanQ_setListRefinement_deq_y: "((\<Gamma>a, CleanQ_Set_deq_y_pre K buf, Language.Basic (CleanQ_Set_deq_y buf)), 
+                               (\<Gamma>c, CleanQ_List_deq_y_pre K buf, Language.Basic (CleanQ_List_deq_y buf)))
+                               \<in> refinement_s (separable_lift sr_set_list fr_id)"
+apply(rule refinement_s_BasicI) (* Problem applying this after unfolding*)
+  unfolding separable_lift_def sr_set_list_def CleanQ_Set_deq_y_def CleanQ_Set_deq_y_pre_def CleanQ_List_deq_y_def
+  CleanQ_List_deq_y_pre_def
+  by(auto)
+
+end
